ITree/Effects/Step.lean
@@ -1,0 +1,58 @@
+import ITree.Effect
+import ITree.Definition
+import ITree.Eval
+import ITree.Exec
+
+namespace ITree.Effects
+
+def stepE : Effect.{u} where
+  I := PUnit
+  O _ := PUnit
+
+def StepE.step {E : Effect.{u}} [stepE -< E] : ITree E PUnit :=
+  .trigger stepE ⟨⟩
+export StepE (step)
+
+section exec
+open ITree.Exec
+
+/- nl is the number of laters per step. First component of the state is
+the number of steps taken so far. Second component of the state is the number of steps left. -/
+def stepEH (nl : Nat → Nat) : SEHandler stepE (ULift.{v} Nat × ULift.{v} Nat) where
+  handle i s p :=
+    nl s.1.down ≤ s.2.down ∧ p ⟨⟩ (ULift.up (s.1.down + 1), ULift.up (s.2.down - nl s.1.down))
+  handle_mono := by grind
+
+theorem exec_step {GE : Effect.{u}} {GR σ p} {s} nl
+    {k : PUnit → ITree GE GR} [stepE -< GE]
+    (eh : EHandler.{u} GE GE GR σ) [hin : InEH (stepEH nl).toEHandler eh]
+    : nl (hin.getState s).1.down ≤ (hin.getState s).2.down →
+      (exec.{u} eh (k ⟨⟩) (hin.putState (ULift.up ((hin.getState s).1.down + 1), ULift.up ((hin.getState s).2.down - nl (hin.getState s).1.down)) s) p) →
+      exec.{u} eh (step >>= k) s p := by
+  intro _ he; unfold step
+  apply exec.dup
+  apply exec.trigger (stepEH nl).toEHandler
+  constructor; assumption
+  simp [he]
+
+theorem exec_step_0 {GE : Effect.{u}} {GR σ p} {s}
+    {k : PUnit → ITree GE GR} [stepE -< GE]
+    (eh : EHandler.{u} GE GE GR σ) [hin : InEH (stepEH λ _ => 0).toEHandler eh]
+    :
+      (exec.{u} eh (k ⟨⟩) (hin.putState (ULift.up ((hin.getState s).1.down + 1), (hin.getState s).2) s) p) →
+      exec.{u} eh (step >>= k) s p := by
+  intro he
+  apply exec_step (λ _ => 0)
+  · simp
+  simp [he]
+
+
+end exec
+
+section eval
+open ITree.Eval
+
+instance stepMH [Monad m] : SMHandler stepE m where
+  handle _ := return ⟨⟩
+
+end eval
